fstar/MLS.Test.Utils.fst
@@ -7,46 +7,7 @@ open Lib.ByteSequence
 open MLS.Result
 open FStar.String
 open MLS.Crypto
-
-val digit_to_string: n:nat{n<10} -> string
-let digit_to_string n =
-  match n with
-  | 0 -> "0"
-  | 1 -> "1"
-  | 2 -> "2"
-  | 3 -> "3"
-  | 4 -> "4"
-  | 5 -> "5"
-  | 6 -> "6"
-  | 7 -> "7"
-  | 8 -> "8"
-  | 9 -> "9"
-
-val nat_to_string: nat -> string
-let rec nat_to_string n =
-  if n < 10 then
-    digit_to_string n
-  else
-    nat_to_string (n/10) ^ digit_to_string (n % 10)
-
-val option_to_string: #a:Type -> (a -> string) -> option a -> string
-let option_to_string #a to_str x =
-  match x with
-  | Some y -> "Some (" ^ (to_str y) ^ ")"
-  | None -> "None"
-
-val list_to_string: #a:Type -> (a -> string) -> list a -> string
-let list_to_string #a to_str l =
-  let rec aux l =
-    match l with
-    | [] -> ""
-    | [x] -> to_str x
-    | h::t -> to_str h ^ "; " ^ aux t
-  in
-  "[" ^ aux l ^ "]"
-
-val string_to_string: string -> string
-let string_to_string s = s
+open MLS.StringUtils
 
 val check_equal: #a:eqtype -> string -> (a -> string) -> a -> a -> ML bool
 let check_equal #a name to_str x y =
@@ -81,35 +42,6 @@ let rec test_list_aux #a test_name test n l =
 val test_list: #a:Type -> string -> (a -> ML bool) -> list a -> ML bool
 let test_list #a test_name test l =
   test_list_aux test_name test 0 l
-
-val hex_digit_to_hex_string: n:nat{n<16} -> string
-let hex_digit_to_hex_string n =
-  match n with
-  | 0 -> "0"
-  | 1 -> "1"
-  | 2 -> "2"
-  | 3 -> "3"
-  | 4 -> "4"
-  | 5 -> "5"
-  | 6 -> "6"
-  | 7 -> "7"
-  | 8 -> "8"
-  | 9 -> "9"
-  | 10 -> "A"
-  | 11 -> "B"
-  | 12 -> "C"
-  | 13 -> "D"
-  | 14 -> "E"
-  | 15 -> "F"
-
-val byte_to_hex_string: n:nat{n<256} -> string
-let byte_to_hex_string n =
-  (hex_digit_to_hex_string (n/16)) ^ (hex_digit_to_hex_string (n%16))
-
-val bytes_to_hex_string: bytes -> string
-let bytes_to_hex_string b =
-  let open Lib.IntTypes in
-  FStar.String.concat "" (List.Tot.map (fun x -> byte_to_hex_string (v x)) (FStar.Seq.seq_to_list b))
 
 val hex_string_to_hex_digit: s:string{strlen s == 1} -> ML (n:nat{n<16})
 let hex_string_to_hex_digit s =
