fstar/MLS.fst
@@ -6,12 +6,16 @@ open MLS.TreeSync.Types
 open MLS.Crypto
 open MLS.NetworkTypes
 open MLS.NetworkBinder
+open MLS.TreeSyncTreeKEMBinder
 open MLS.TreeSync.Extensions
+open MLS.TreeSync.ExternalPath
+open MLS.TreeKEM
 open MLS.TreeDEM.Message.Types
 open MLS.TreeDEM.Message.Content
 open MLS.TreeDEM.Message.Framing
 open MLS.TreeDEM.Welcome
 open MLS.Parser
+open MLS.Utils
 open MLS.Result
 
 #set-options "--fuel 0 --ifuel 0"
@@ -32,12 +36,14 @@ type state = {
   cs: ciphersuite;
   tree_state: s:MLS.TreeSync.Types.state_t;
   leaf_index: nat;
+  leaf_secret: bytes;
   sign_private_key: sign_private_key cs;
   handshake_state: MLS.TreeDEM.Keys.ratchet_state cs;
   application_state: MLS.TreeDEM.Keys.ratchet_state cs;
   epoch_secret: bytes;
   confirmed_transcript_hash: bytes;
   interim_transcript_hash: bytes;
+  pending_updatepath: list (bytes & bytes); //key_package & leaf_secret
 }
 
 #push-options "--fuel 1"
@@ -67,6 +73,13 @@ val state_to_group_context: state -> result group_context_nt
 let state_to_group_context st =
   compute_group_context st.tree_state.group_id st.tree_state.version st.tree_state.tree st.confirmed_transcript_hash
 
+val hash_leaf_package: leaf_package_t -> result bytes
+let hash_leaf_package leaf_package =
+  key_package <-- treesync_to_keypackage cs leaf_package;
+  let key_package = ps_key_package.serialize key_package in
+  hash <-- hash_hash cs key_package;
+  return (hash <: bytes)
+
 #push-options "--fuel 1"
 val reset_ratchet_states: state -> result state
 let reset_ratchet_states st =
@@ -82,49 +95,128 @@ let reset_ratchet_states st =
   )
 #pop-options
 
+val process_proposal: nat -> state -> proposal -> result state
+let process_proposal sender_id st p =
+  sender_cred <-- (
+    if not (sender_id < st.tree_state.treesize) then
+      error "process_proposal: sender_id is greater than treesize"
+    else (
+      let (_, opt_sender_leaf_package) = get_leaf st.tree_state.tree sender_id in
+      if not (Some? opt_sender_leaf_package) then
+        error "process_proposal: sender_id points to a blank leaf"
+      else
+        return (Some?.v opt_sender_leaf_package).credential
+    )
+  );
+  match p with
+  | Add leaf_package ->
+    let (tree_state, _) = MLS.TreeSync.add st.tree_state sender_cred leaf_package in
+    return ({ st with tree_state })
+  | Update leaf_package ->
+    if not (sender_id < st.tree_state.treesize) then
+      error "process_proposal: leaf_ind is greater than treesize"
+    else (
+      let tree_state = MLS.TreeSync.update st.tree_state sender_cred leaf_package sender_id in
+      return ({ st with tree_state })
+    )
+  | Remove leaf_ind ->
+    if not (leaf_ind < st.tree_state.treesize) then
+      error "process_proposal: sender_id is greater than treesize"
+    else (
+      let tree_state = MLS.TreeSync.remove st.tree_state sender_cred leaf_ind in
+      return ({ st with tree_state })
+    )
+  | _ -> error "process_proposal: not implemented"
+
+val process_proposals: state -> nat -> list proposal -> result state
+let process_proposals st sender_id proposals =
+  let sorted_proposals = List.Tot.concatMap (fun x -> x) [
+    List.Tot.filter (Update?) proposals;
+    List.Tot.filter (Remove?) proposals;
+    List.Tot.filter (Add?) proposals;
+    List.Tot.filter (fun x -> match x with | Add _ | Update _ | Remove _ -> false | _ -> true) proposals;
+  ] in
+  fold_leftM (process_proposal sender_id) st sorted_proposals
+
+#push-options "--ifuel 1"
+val proposal_or_ref_to_proposal: state -> proposal_or_ref -> result proposal
+let proposal_or_ref_to_proposal st prop_or_ref =
+  match prop_or_ref with
+  | Proposal prop -> return prop
+  | Reference ref -> error "proposal_or_ref_to_proposal: don't handle references for now (TODO)"
+#pop-options
+
 val process_commit: state -> msg:message{msg.content_type = CT_commit} -> message_auth -> result (state & bytes)
 let process_commit state message message_auth =
   let message: MLS.TreeDEM.Message.Types.message = message in
   let message_content: commit = message.message_content in
-  match message_content with
-  | { c_proposals = [ Proposal (Add leaf_package) ]; c_path = None } ->
-      // SKETCH...
-      let sender_id = message.sender.sender_id in
-      // let sender_cred = find_credentials state.tree sender_id in
-      let sender_cred = MLS.NetworkBinder.dumb_credential in
-      // 1. Process addition to the tree
-      let (tree_state, _) = MLS.TreeSync.add state.tree_state sender_cred leaf_package in
-      let state = { state with tree_state } in
-      // 2. Increase epoch -- TODO when should this happen?!!
-      let tree_state = { tree_state with version = tree_state.version + 1 } in
-      // 3. Update transcript
-      confirmed_transcript_hash <-- MLS.TreeDEM.Message.Transcript.compute_confirmed_transcript_hash
-        cs message message_auth.signature state.interim_transcript_hash;
-      interim_transcript_hash <-- MLS.TreeDEM.Message.Transcript.compute_interim_transcript_hash
-        cs message_auth.confirmation_tag confirmed_transcript_hash;
-      let state = { state with confirmed_transcript_hash; interim_transcript_hash } in
-      // 4. New group context
+  let sender_id = message.sender.sender_id in
+  // 0. Process proposals
+  proposals <-- mapM (proposal_or_ref_to_proposal state) message_content.c_proposals;
+  state <-- process_proposals state sender_id proposals;
+  // 1. Process update path
+  state <-- (
+    match message_content.c_path with
+    | None -> return state
+    | Some path ->
       group_context <-- state_to_group_context state;
-      // 5. Ratchet.
-      init_secret <-- MLS.TreeDEM.Keys.secret_epoch_to_init cs state.epoch_secret;
-      let commit_secret = Seq.create 32 (Lib.IntTypes.u8 0) in // FIXME if c_path <> None
-      joiner_secret <-- MLS.TreeDEM.Keys.secret_init_to_joiner cs init_secret commit_secret;
-      let psk_secret = bytes_empty in
-      let serialized_group_context = ps_group_context.serialize group_context in
-      epoch_secret <-- MLS.TreeDEM.Keys.secret_joiner_to_epoch cs joiner_secret psk_secret serialized_group_context;
-      let state = { state with epoch_secret } in
-      state <-- reset_ratchet_states state;
-      // - then maybe something like this once we gain the ability to process c_path = Some update_path...?
-      (*group_context <-- state_to_group_context state;
-      update_pathkem <-- update_path_to_treekem cs state.tree_state.level state.tree_state.treesize
-        sender_id group_context update_path;
-      update_leaf_package <-- key_package_to_treesync leaf_package;
-      ext_ups1 <-- MLS.TreeSyncTreeKEMBinder.treekem_to_treesync leaf_package update_pathkem;
-      let ups1 = extract_result (external_pathsync_to_pathsync cs None ts1 ext_ups1) in
-      let ts2 = apply_path dumb_credential ts1 ups1 in
-      let tk2 = extract_result (treesync_to_treekem cs ts2) in*)
-      return (state, (joiner_secret <: bytes))
-  | _ -> internal_failure "TODO: commit (general case)"
+      let group_context_bytes = ps_group_context.serialize group_context in
+      //It is not possible to move this `if` inside the definition of `update_pathkem`, because we need the information it gives to write the type of `update_pathkem`
+      if not (sender_id < state.tree_state.treesize) then
+        error "process_commit: sender_id is greater than treesize"
+      else (
+        update_pathkem <-- update_path_to_treekem cs state.tree_state.levels state.tree_state.treesize sender_id group_context_bytes path;
+        update_leaf_package <-- key_package_to_treesync path.leaf_key_package;
+        ext_update_pathsync <-- treekem_to_treesync update_leaf_package update_pathkem;
+        update_pathsync <-- external_pathsync_to_pathsync cs None state.tree_state.tree ext_update_pathsync;
+        return ({ state with
+          tree_state = { state.tree_state with
+            tree = MLS.TreeSync.apply_path dumb_credential state.tree_state.tree update_pathsync;
+          }
+        })
+      )
+  );
+  // 2. Increase epoch -- TODO when should this happen?!!
+  let tree_state = state.tree_state in
+  let tree_state = { tree_state with version = tree_state.version + 1 } in
+  let state = { state with tree_state } in
+  // 3. Update transcript
+  confirmed_transcript_hash <-- MLS.TreeDEM.Message.Transcript.compute_confirmed_transcript_hash
+    cs message message_auth.signature state.interim_transcript_hash;
+  interim_transcript_hash <-- MLS.TreeDEM.Message.Transcript.compute_interim_transcript_hash
+    cs message_auth.confirmation_tag confirmed_transcript_hash;
+  let state = { state with confirmed_transcript_hash; interim_transcript_hash } in
+  // 4. New group context
+  group_context <-- state_to_group_context state;
+  // 5. Ratchet.
+  init_secret <-- MLS.TreeDEM.Keys.secret_epoch_to_init cs state.epoch_secret;
+  leaf_secret <-- (
+    if state.leaf_index = sender_id && (Some? message_content.c_path) then (
+      match List.Tot.assoc (ps_key_package.serialize (Some?.v message_content.c_path).leaf_key_package) state.pending_updatepath with
+      | Some leaf_secret -> return leaf_secret
+      | None -> internal_failure "Can't retrieve my own leaf secret"
+    ) else (
+      return state.leaf_secret
+    )
+  );
+  commit_secret <-- (
+    match message_content.c_path with
+    | None -> return (Seq.create 32 (Lib.IntTypes.u8 0))
+    | Some _ ->
+      if not (state.leaf_index < state.tree_state.treesize) then
+        error "process_commit: leaf index is too big"
+      else (
+        tree <-- treesync_to_treekem cs state.tree_state.tree;
+        MLS.TreeKEM.root_secret tree state.leaf_index leaf_secret
+      )
+  );
+  joiner_secret <-- MLS.TreeDEM.Keys.secret_init_to_joiner cs init_secret commit_secret;
+  let psk_secret = bytes_empty in
+  let serialized_group_context = ps_group_context.serialize group_context in
+  epoch_secret <-- MLS.TreeDEM.Keys.secret_joiner_to_epoch cs joiner_secret psk_secret serialized_group_context;
+  let state = { state with epoch_secret; leaf_secret; pending_updatepath = [];} in
+  state <-- reset_ratchet_states state;
+  return (state, (joiner_secret <: bytes))
 
 let fresh_key_pair e =
   if not (Seq.length e = sign_private_key_length cs) then
@@ -141,12 +233,13 @@ let chop_entropy (e: bytes) (l: nat): (result ((fresh:bytes{Seq.length fresh == 
     let (fresh, next) = (Seq.split e l) in
     return (fresh, next)
 
+val fresh_key_package_internal: e:entropy { Seq.length e == 64 } -> credential -> MLS.Crypto.sign_private_key cs -> result (leaf_package_t & bytes)
 let fresh_key_package_internal e { identity; signature_key } private_sign_key =
-  tmp <-- chop_entropy e (hpke_private_key_length cs);
+  tmp <-- chop_entropy e (kdf_length cs);
   let fresh, e = tmp in
-  // TODO: debug this and the other occurrence below
-  key_pair <-- hpke_gen_keypair cs fresh;
-  let ((private_key: bytes), public_key) = key_pair in
+  let leaf_secret = fresh in
+  key_pair <-- MLS.TreeKEM.derive_keypair_from_path_secret cs leaf_secret;
+  let (_, public_key) = key_pair in
   extensions <-- (
     let versions = Seq.seq_of_list [PV_mls10] in
     let ciphersuites = Seq.seq_of_list [CS_mls10_128_dhkemx25519_chacha20poly1305_sha256_ed25519] in
@@ -182,24 +275,24 @@ let fresh_key_package_internal e { identity; signature_key } private_sign_key =
     sign_sign cs private_sign_key tbs nonce
   );
   let leaf_package = { unsigned_leaf_package with signature } in
-  return (leaf_package, private_key)
+  return (leaf_package, (leaf_secret <: bytes))
 
 let fresh_key_package e cred private_sign_key =
   tmp <-- fresh_key_package_internal e cred private_sign_key;
-  let leaf_package, private_key = tmp in
+  let leaf_package, leaf_secret = tmp in
   key_package <-- treesync_to_keypackage cs leaf_package;
   let key_package = ps_key_package.serialize key_package in
-  hash <-- hash_hash cs key_package;
-  return (key_package, hash, private_key)
+  hash <-- hash_leaf_package leaf_package;
+  return (key_package, hash, leaf_secret)
 
 let current_epoch s = s.tree_state.MLS.TreeSync.Types.version
 
-#push-options "--fuel 2"
+#push-options "--fuel 2 --z3rlimit 50"
 let create e cred private_sign_key group_id =
   tmp <-- chop_entropy e 64;
   let fresh, e = tmp in
   tmp <-- fresh_key_package_internal fresh cred private_sign_key;
-  let leaf_package, private_key = tmp in
+  let leaf_package, leaf_secret = tmp in
   let tree_state = MLS.TreeSync.create group_id leaf_package in
   // 10. In principle, the above process could be streamlined by having the
   // creator directly create a tree and choose a random value for first epoch's
@@ -207,19 +300,21 @@ let create e cred private_sign_key group_id =
   tmp <-- chop_entropy e 32;
   let epoch_secret, e = tmp in
   encryption_secret <-- MLS.TreeDEM.Keys.secret_epoch_to_encryption cs epoch_secret;
-  leaf_secret <-- MLS.TreeDEM.Keys.leaf_kdf #0 1 cs encryption_secret 0 0;
-  handshake_state <-- MLS.TreeDEM.Keys.init_handshake_ratchet cs 0 leaf_secret;
-  application_state <-- MLS.TreeDEM.Keys.init_application_ratchet cs 0 leaf_secret;
+  leaf_dem_secret <-- MLS.TreeDEM.Keys.leaf_kdf #0 1 cs encryption_secret 0 0;
+  handshake_state <-- MLS.TreeDEM.Keys.init_handshake_ratchet cs 0 leaf_dem_secret;
+  application_state <-- MLS.TreeDEM.Keys.init_application_ratchet cs 0 leaf_dem_secret;
   return ({
     cs;
     tree_state;
     leaf_index = 0;
+    leaf_secret;
     sign_private_key = private_sign_key;
     handshake_state;
     application_state;
     epoch_secret;
     confirmed_transcript_hash = Seq.empty;
     interim_transcript_hash = Seq.empty;
+    pending_updatepath = [];
   })
 #pop-options
 
@@ -242,28 +337,11 @@ let send_helper st msg e =
   let g:group_message = (st.tree_state.group_id, msg_bytes) in
   return (new_st, auth, g)
 
-#push-options "--fuel 2 --ifuel 2 --z3rlimit 20"
-let add state key_package e =
-  kp <-- from_option "error message if it is malformed" ((ps_to_pse ps_key_package).parse_exact key_package);
-  lp <-- key_package_to_treesync kp;
-  let msg: message = {
-    group_id = (state.tree_state <: state_t).group_id;
-    epoch = (state.tree_state <: state_t).version;
-    sender = {
-      sender_type = ST_member;
-      sender_id = state.leaf_index;
-    };
-    authenticated_data = Seq.empty; //TODO?
-    content_type = CT_commit;
-    message_content = { c_proposals = [ Proposal (Add lp) ]; c_path = None };
-  } in
-  tmp <-- chop_entropy e 4;
-  let fresh, e = tmp in
-  tmp <-- send_helper state msg fresh;
-  let (new_state, msg_auth, g) = tmp in
-  tmp <-- process_commit new_state msg msg_auth;
+val generate_welcome_message: state -> msg:message{msg.content_type == CT_commit} -> message_auth -> bool -> new_leaf_packages:list leaf_package_t -> randomness (let open FStar.Mul in (List.Tot.length new_leaf_packages)*(hpke_private_key_length cs)) -> result welcome
+let generate_welcome_message st msg msg_auth include_path_secrets new_leaf_packages rand =
+  tmp <-- process_commit st msg msg_auth;
   let (future_state, joiner_secret) = tmp in
-  confirmation_tag <-- from_option "" msg_auth.confirmation_tag;
+  confirmation_tag <-- from_option "generate_welcome_message: confirmation tag is missing" msg_auth.confirmation_tag;
   tree_hash <-- MLS.TreeSync.Hash.tree_hash future_state.cs (MLS.TreeMath.root future_state.tree_state.levels) future_state.tree_state.tree;
   ratchet_tree <-- treesync_to_ratchet_tree cs future_state.tree_state.tree;
   ratchet_tree_bytes <-- (
@@ -271,35 +349,146 @@ let add state key_package e =
     if 1 <= l && l < pow2 32 then
       return (ps_ratchet_tree.serialize ratchet_tree)
     else
-      internal_failure "add: ratchet_tree too big"
+      internal_failure "generate_welcome_message: ratchet_tree too big"
   );
   let group_info: welcome_group_info = {
-    group_id = state.tree_state.group_id;
+    group_id = future_state.tree_state.group_id;
     epoch = future_state.tree_state.version;
     tree_hash = tree_hash;
     confirmed_transcript_hash = future_state.confirmed_transcript_hash;
     extensions = ratchet_tree_bytes;
     confirmation_tag = confirmation_tag;
-    signer_index = state.leaf_index;
-    signature = Seq.empty;
+    signer_index = future_state.leaf_index;
+    signature = Seq.empty; //TODO
   } in
-  assume (hpke_private_key_length cs == 32);
-  tmp <-- chop_entropy e 32;
-  let fresh, e = tmp in
-  let rand: randomness (hpke_private_key_length cs) = (mk_randomness #32 fresh) in
-  welcome_msg <-- encrypt_welcome cs group_info joiner_secret [(lp, None)] rand;
-  welcome_msg_network <-- welcome_to_network cs welcome_msg;
-  let w:welcome_message = (Seq.empty, ps_welcome.serialize welcome_msg_network) in
-  return (new_state, (g,w))
+  leaf_packages_and_path_secrets <-- mapM (fun new_leaf_package ->
+    if Some? (msg <: message).message_content.c_path then (
+      match find_first (fun (_, lp) -> lp = Some (new_leaf_package)) (get_leaf_list future_state.tree_state.tree) with
+      | None -> internal_failure "generate_welcome_message: can't find newly added leaf package"
+      | Some new_leaf_index ->
+        if not (future_state.leaf_index < future_state.tree_state.treesize) then
+          internal_failure "generate_welcome_message: state leaf index is too big"
+        else if not (new_leaf_index <> future_state.leaf_index) then
+          internal_failure "generate_welcome_message: new leaf index is equal to our leaf index"
+        else (
+          tk <-- treesync_to_treekem cs future_state.tree_state.tree;
+          path_secret <-- path_secret_at_least_common_ancestor tk future_state.leaf_index new_leaf_index future_state.leaf_secret;
+          return (new_leaf_package, Some path_secret)
+        )
+    ) else (
+      return (new_leaf_package, None)
+    )
+  ) new_leaf_packages;
+  assume (List.Tot.length leaf_packages_and_path_secrets == List.Tot.length new_leaf_packages);
+  welcome_msg <-- encrypt_welcome cs group_info joiner_secret leaf_packages_and_path_secrets rand;
+  return welcome_msg
+
+#push-options "--ifuel 2 --fuel 2 --z3rlimit 30"
+val generate_update_path: state -> bytes -> list proposal -> result (update_path_nt & (bytes & bytes) & bytes)
+let generate_update_path st e proposals =
+  // TODO: MLS' spec impose to exclude newly added leaves from the resolution computation.
+  // This is because the path secret is already encrypted to these leaves in the Welcome message
+  // This is an optimization to use one less encryption/decryption for the sender and the added participant, for each added participant
+  // (There in only one encryption in the welcome message, instead of two in the welcome message and in the update path)
+  // This optimization (necessary for interop) is currently not implemented
+  // It also needs to be implemented in `process_commit`.
+  // This is the reason of processing the proposals here, since we need to know which leaves will be added
+  st <-- process_proposals st st.leaf_index proposals; //This will be more complex in the future, or maybe process_proposals will give the indices of new leaves?
+  tree_kem <-- treesync_to_treekem cs st.tree_state.tree;
+  if not (st.leaf_index < st.tree_state.treesize) then
+    internal_failure "generate_update_path: leaf index is too big"
+  else (
+    let update_path_entropy = update_path_entropy_length tree_kem st.leaf_index in
+    assume (update_path_entropy < pow2 32); //MEH
+    tmp <-- chop_entropy e update_path_entropy;
+    let fresh, e = tmp in
+    let update_path_rand = mk_randomness #update_path_entropy fresh in
+    tmp <-- chop_entropy e (sign_nonce_length st.cs);
+    let fresh, e = tmp in
+    let sign_nonce = mk_randomness #(sign_nonce_length st.cs) fresh in
+    group_context <-- state_to_group_context st;
+    let group_context_bytes = ps_group_context.serialize group_context in
+    let new_leaf_secret = Seq.create (hpke_private_key_length cs) (Lib.IntTypes.u8 0)  in
+    tmp <-- update_path tree_kem st.leaf_index new_leaf_secret group_context_bytes update_path_rand;
+    let (update_path_kem, _) = tmp in
+    let (_, opt_my_leaf_package) =  get_leaf st.tree_state.tree st.leaf_index in
+    my_leaf_package <-- (from_option "generate_update_path: my leaf is blanked" opt_my_leaf_package);
+    update_path_ext_sync <-- treekem_to_treesync my_leaf_package update_path_kem;
+    update_path_sync <-- external_pathsync_to_pathsync st.cs (Some (st.sign_private_key, sign_nonce)) st.tree_state.tree update_path_ext_sync;
+    update_path_network <-- treesync_to_update_path cs update_path_sync;
+    let new_key_package_bytes = ps_key_package.serialize update_path_network.leaf_key_package in
+    return (update_path_network, (new_key_package_bytes, new_leaf_secret), e)
+  )
 #pop-options
 
-let remove state p = admit()
-let update state e = admit()
+let message_commit = m:message{m.content_type == CT_commit}
+
+val generate_commit: state -> entropy -> list proposal -> result (message_commit & state & entropy)
+let generate_commit state e proposals =
+  tmp <-- generate_update_path state e proposals;
+  let (update_path, pending, e) = tmp in
+  let state = { state with pending_updatepath = pending::state.pending_updatepath} in
+  let msg: message = {
+    group_id = state.tree_state.group_id;
+    epoch = state.tree_state.version;
+    sender = {
+      sender_type = ST_member;
+      sender_id = state.leaf_index;
+    };
+    authenticated_data = Seq.empty; //TODO?
+    content_type = CT_commit;
+    message_content = { c_proposals = (List.Tot.map Proposal proposals); c_path = Some update_path };
+  } in
+  return ((msg <: message_commit), state, e)
+
+let add state key_package e =
+  kp <-- from_option "error message if it is malformed" ((ps_to_pse ps_key_package).parse_exact key_package);
+  lp <-- key_package_to_treesync kp;
+  let proposals = [ (Add lp) ] in
+  tmp <-- generate_commit state e proposals;
+  let (msg, state, e) = tmp in
+  tmp <-- chop_entropy e 4;
+  let fresh, e = tmp in
+  tmp <-- send_helper state msg fresh;
+  let (state, msg_auth, g) = tmp in
+  tmp <-- chop_entropy e 32;
+  let fresh, e = tmp in
+  let rand = mk_randomness #32 fresh in
+  assume (hpke_private_key_length cs == 32);
+  assert_norm (List.Tot.length [lp] == 1);
+  welcome_msg <-- generate_welcome_message state msg msg_auth false [lp] rand;
+  welcome_msg_network <-- welcome_to_network cs welcome_msg;
+  let w:welcome_message = (Seq.empty, ps_welcome.serialize welcome_msg_network) in
+  return (state, (g,w))
+
+let remove state p e =
+  match find_first (fun (_, olp) -> match olp with | Some lp -> (lp <: leaf_package_t).credential.identity = p | None -> false) (get_leaf_list state.tree_state.tree) with
+  | None -> error "remove: can't find the leaf to remove"
+  | Some i -> (
+    let proposals = [Remove i] in
+    tmp <-- generate_commit state e proposals;
+    let (msg, state, e) = tmp in
+    tmp <-- chop_entropy e 4;
+    let fresh, e = tmp in
+    tmp <-- send_helper state msg fresh;
+    let (state, _, g) = tmp in
+    return (state, g)
+  )
+
+let update state e =
+  let proposals = [] in
+  tmp <-- generate_commit state e proposals;
+  let (msg, state, e) = tmp in
+  tmp <-- chop_entropy e 4;
+  let fresh, e = tmp in
+  tmp <-- send_helper state msg fresh;
+  let (state, _, g) = tmp in
+  return (state, g)
 
 let send state e data =
   let msg: message = {
-    group_id = (state.tree_state <: state_t).group_id;
-    epoch = (state.tree_state <: state_t).version;
+    group_id = state.tree_state.group_id;
+    epoch = state.tree_state.version;
     sender = {
       sender_type = ST_member;
       sender_id = state.leaf_index;
@@ -313,20 +502,6 @@ let send state e data =
   return (new_state, g)
 
 
-// FIXME this is a copy
-val find_first: #a:Type -> (a -> bool) -> l:list a -> option (n:nat{n < List.Tot.length l})
-let rec find_first #a p l =
-  match l with
-  | [] -> None
-  | h::t ->
-    if p h then (
-      Some 0
-    ) else (
-      match find_first p t with
-      | Some v -> Some (v+1)
-      | None -> None
-    )
-
 val find_my_index: #l:nat -> #n:tree_size l -> treesync l n -> bytes -> result (res:nat{res<n})
 let find_my_index #l #n t sign_pk =
   let test (oc: option credential_t) =
@@ -336,25 +511,58 @@ let find_my_index #l #n t sign_pk =
   in
   from_option "couldn't find my_index" (find_first test (Seq.seq_to_list (MLS.TreeSync.tree_membership t)))
 
-#push-options "--fuel 1"
+#push-options "--fuel 1 --z3rlimit 50"
 let process_welcome_message w (sign_pk, sign_sk) lookup =
   let (_, welcome_bytes) = w in
-  welcome_network <-- from_option "" ((ps_to_pse ps_welcome).parse_exact welcome_bytes);
+  welcome_network <-- from_option "process_welcome_message: can't parse welcome message" ((ps_to_pse ps_welcome).parse_exact welcome_bytes);
   let welcome = network_to_welcome welcome_network in
   tmp <-- decrypt_welcome cs welcome (fun kp_hash ->
     match lookup kp_hash with
-    | Some sk -> if Seq.length sk = hpke_private_key_length cs then Some sk else None
+    | Some leaf_secret -> (
+      //TODO: here we break result's encapsulation
+      match MLS.TreeKEM.derive_keypair_from_path_secret cs leaf_secret with
+      | Success (sk, _) -> Some sk
+      | _ -> None
+    )
     | None -> None
   ) None;
   let (group_info, secrets) = tmp in
   ratchet_tree <-- from_option "bad ratchet tree" ((ps_to_pse ps_ratchet_tree).parse_exact group_info.extensions);
   ln <-- ratchet_tree_l_n ratchet_tree;
   let (|l, n|) = ln in
-  ts <-- ratchet_tree_to_treesync l n ratchet_tree;
+  tree <-- ratchet_tree_to_treesync l n ratchet_tree;
+  leaf_index <-- find_my_index tree sign_pk;
+  tree <-- (
+    match secrets.path_secret with
+    | None -> return tree
+    | Some path_secret ->
+      if not (group_info.signer_index <> leaf_index) then
+        error "process_welcome_message: signer index is equal to our leaf index"
+      else if not (group_info.signer_index < n) then
+        error "process_welcome_message: signer index is too big"
+      else (
+        tree_kem <-- treesync_to_treekem cs tree;
+        update_path_kem <-- mk_init_path tree_kem leaf_index group_info.signer_index path_secret bytes_empty;
+        sender_leaf_package <-- from_option "process_welcome_message: signer leaf is blanked" (snd (get_leaf tree group_info.signer_index));
+        external_update_path <-- treekem_to_treesync sender_leaf_package update_path_kem;
+        update_path <-- external_pathsync_to_pathsync cs None tree external_update_path;
+        return (MLS.TreeSync.apply_path sender_leaf_package.credential tree update_path)
+      )
+  );
   interim_transcript_hash <-- MLS.TreeDEM.Message.Transcript.compute_interim_transcript_hash cs (Some group_info.confirmation_tag) group_info.confirmed_transcript_hash;
-  group_context <-- compute_group_context group_info.group_id group_info.epoch ts group_info.confirmed_transcript_hash;
+  group_context <-- compute_group_context group_info.group_id group_info.epoch tree group_info.confirmed_transcript_hash;
   epoch_secret <-- MLS.TreeDEM.Keys.secret_joiner_to_epoch cs secrets.joiner_secret bytes_empty (ps_group_context.serialize group_context);
-  leaf_index <-- find_my_index ts sign_pk;
+  leaf_secret <-- (
+    let opt_my_leaf_package = get_leaf tree leaf_index in
+    match opt_my_leaf_package with
+    | (_, None) -> internal_failure "process_welcome_message: leaf index points to a blank leaf"
+    | (_, Some my_leaf_package) -> (
+      kp_hash <-- hash_leaf_package my_leaf_package;
+      match lookup kp_hash with
+      | Some leaf_secret -> return leaf_secret
+      | None -> internal_failure "process_welcome_message: decrypt_welcome found my leaf package but not proccess_welcome_message"
+    )
+  );
   let dumb_ratchet_state: MLS.TreeDEM.Keys.ratchet_state cs = {
     secret = Seq.create (kdf_length cs) (Lib.IntTypes.u8 0);
     generation = 0;
@@ -366,22 +574,23 @@ let process_welcome_message w (sign_pk, sign_sk) lookup =
       group_id = group_info.group_id;
       levels = l;
       treesize = n;
-      tree = ts;
+      tree;
       version = group_info.epoch;
       transcript = Seq.empty;
     };
     leaf_index;
+    leaf_secret;
     sign_private_key = sign_sk;
     handshake_state = dumb_ratchet_state;
     application_state = dumb_ratchet_state;
     epoch_secret;
     confirmed_transcript_hash = group_info.confirmed_transcript_hash;
     interim_transcript_hash;
+    pending_updatepath = [];
   } in
   st <-- reset_ratchet_states st;
   return(group_info.group_id, st)
 #pop-options
-
 
 let process_group_message state msg =
   msg <-- from_option "process_group_message: can't parse group message"
@@ -413,7 +622,7 @@ let process_group_message state msg =
   | MLS.TreeDEM.Message.Content.CT_commit ->
       let message_content: commit = message.message_content in
       begin match message_content with
-      | { c_proposals = [ Proposal (Add leaf_package) ]; c_path = None } ->
+      | { c_proposals = [ Proposal (Add leaf_package) ]; c_path = _ } ->
           tmp <-- process_commit state message message_auth;
           let (state, _) = tmp in
           return (state, MsgAdd leaf_package.credential.identity)
